eliminate type_weaken
- type_weaken is not implementable when types are not total, or
  we just need an appropriate default.

theories/EnvI.v
@@ -11,21 +11,21 @@ Section Env.
   Variable typ : Type.
   Context {RType_typ : RType typ}.
 
+  Variable ts : list Type.
+
   (** Environments **)
   Definition tenv : Type := list typ.
-  Definition env : Type := list (sigT (typD nil)).
+  Definition env : Type := list (sigT (typD ts)).
 
   Definition typeof_env (e : env) : tenv :=
     map (@projT1 _ _) e.
-
-  Variable ts : list Type.
 
   Definition lookupAs (e : env) (n : nat) (ty : typ) : option (typD ts ty) :=
     match nth_error e n with
       | None => None
       | Some (existT t v) =>
         match type_cast ts ty t with
-          | Some pf => Some (Relim (fun x => x) pf (type_weaken ts t v))
+          | Some pf => Some (Relim (fun x => x) pf v)
           | None => None
         end
     end.
@@ -39,13 +39,13 @@ Section Env.
     erewrite nth_error_weaken by eassumption. auto.
   Qed.
 
-  Fixpoint join_env (gs : list typ) (hgs : hlist (typD nil) gs) : env :=
+  Fixpoint join_env (gs : list typ) (hgs : hlist (typD ts) gs) : env :=
     match hgs with
       | Hnil => nil
       | Hcons a b c d => existT _ _ c :: join_env d
     end.
 
-  Fixpoint split_env (gs : env) : sigT (hlist (typD nil)) :=
+  Fixpoint split_env (gs : env) : sigT (hlist (typD ts)) :=
     match gs with
       | nil => existT _ nil Hnil
       | g :: gs =>
@@ -83,7 +83,7 @@ Section Env.
     nth_error ve v = Some tv <->
     match nth_error (projT1 (split_env ve)) v as t
           return match t with
-                   | Some v => typD nil v
+                   | Some v => typD ts v
                    | None => unit
                  end -> Prop
     with
@@ -319,6 +319,6 @@ Section nth_error_get_hlist_nth.
 
 End nth_error_get_hlist_nth.
 
-Arguments env {typ _} : rename.
-Arguments join_env {_ _ _} _.
-Arguments split_env {_ _} _.
+Arguments env {typ _} _ : rename.
+Arguments join_env {typ _ _ _} _ : rename.
+Arguments split_env {typ _ _} _ : rename.
